commit before changing [] to getI

Computability/Constructions/CovRec.lean
@@ -1,157 +1,8 @@
 import Computability.Constructions.Basic
 import Computability.Constructions.List
+
 open Nat.RecursiveIn.Code
-
-section l_append
-def Nat.list_append (list index:ℕ):ℕ:=Nat.pair (list.l+1) $ Nat.pair list.r index
-namespace Nat.RecursiveIn.Code
-def c_l_append := pair (succ.comp $ left.comp left) (pair (right.comp left) right)
-@[simp] theorem c_l_append_ev_pr:code_prim c_l_append := by unfold c_l_append; repeat (first|assumption|simp|constructor)
-@[simp] theorem c_l_append_evp:eval_prim O c_l_append = unpaired2 Nat.list_append := by unfold Nat.list_append; simp [c_l_append,eval_prim];
-@[simp] theorem c_l_append_ev:eval O c_l_append = unpaired2 Nat.list_append := by rw [← eval_prim_eq_eval c_l_append_ev_pr]; simp only [c_l_append_evp]
-end Nat.RecursiveIn.Code
--- theorem Nat.PrimrecIn.l_append:Nat.PrimrecIn O Nat.l_append := by ...
--- theorem Nat.Primrec.l_append:Nat.Primrec Nat.l_append := by ...
-end l_append
-
-section l_get_last
-def Nat.list_get_last_aux (list index:ℕ):ℕ:=
-  match index with
-  | 0 => list.r
-  | Nat.succ prev_index => (Nat.list_get_last_aux list prev_index).l
-def Nat.list_get_lastn (list index:ℕ):ℕ:=(Nat.list_get_last_aux list index).r
-def Nat.list_get_last (list:ℕ) :=list.r.r
-def Nat.list_size (list:ℕ) := list.l
-def Nat.list_get (list index:ℕ) := Nat.list_get_lastn list (list.list_size-1-index)
-
-#check (Nat.pair 2 (Nat.pair (Nat.pair 0 132) 42))
-#eval Nat.list_get_last (Nat.pair 2 (Nat.pair (Nat.pair 0 132) 42))
-#eval Nat.list_get_lastn (Nat.pair 2 (Nat.pair (Nat.pair 0 132) 42)) 0
-#eval Nat.list_get_lastn (Nat.pair 2 (Nat.pair (Nat.pair 0 132) 42)) 1
-
-namespace Nat.RecursiveIn.Code
-def c_l_get_lastn_aux := prec right (left.comp $ right.comp right)
-@[simp] theorem c_l_get_lastn_aux_ev_pr:code_prim c_l_get_lastn_aux := by unfold c_l_get_lastn_aux; repeat (first|assumption|simp|constructor)
-@[simp] theorem c_l_get_lastn_aux_evp:eval_prim O c_l_get_lastn_aux = unpaired2 Nat.list_get_last_aux := by
-  simp [c_l_get_lastn_aux,eval_prim];
-  funext n;
-  simp [unpaired2]
-  induction n.r with
-  | zero => exact rfl
-  | succ n h => exact congrArg Prod.fst (congrArg unpair h)
-@[simp] theorem c_l_get_lastn_aux_ev:eval O c_l_get_lastn_aux = unpaired2 Nat.list_get_last_aux := by rw [← eval_prim_eq_eval c_l_get_lastn_aux_ev_pr]; simp only [c_l_get_lastn_aux_evp];
-
-def c_l_get_lastn := right.comp c_l_get_lastn_aux
-@[simp] theorem c_l_get_lastn_ev_pr:code_prim c_l_get_lastn := by unfold c_l_get_lastn; repeat (first|assumption|simp|constructor)
-@[simp] theorem c_l_get_lastn_evp:eval_prim O c_l_get_lastn = unpaired2 Nat.list_get_lastn := by
-  unfold list_get_lastn
-  simp [c_l_get_lastn,eval_prim];
-@[simp] theorem c_l_get_lastn_ev:eval O c_l_get_lastn = unpaired2 Nat.list_get_lastn := by rw [← eval_prim_eq_eval c_l_get_lastn_ev_pr]; simp only [c_l_get_lastn_evp];
-
-def c_l_get_last := c_l_get_lastn.comp₂ c_id (c_const 0)
-@[simp] theorem c_l_get_last_ev_pr:code_prim c_l_get_last := by unfold c_l_get_last; repeat (first|assumption|simp|constructor);
-@[simp] theorem c_l_get_last_evp:eval_prim O c_l_get_last = Nat.list_get_last := by
-  unfold list_get_last
-  simp [c_l_get_last,eval_prim];
-  exact rfl
-@[simp] theorem c_l_get_last_ev:eval O c_l_get_last = Nat.list_get_last := by rw [← eval_prim_eq_eval c_l_get_last_ev_pr]; simp only [c_l_get_last_evp];
-end Nat.RecursiveIn.Code
--- theorem Nat.PrimrecIn.l_get:Nat.PrimrecIn O Nat.l_get := by ...
--- theorem Nat.Primrec.l_get:Nat.Primrec Nat.l_get := by ...
-end l_get_last
-
-
--- takes a pair (list,index)
-section l_get
-namespace Nat.RecursiveIn.Code
-def c_l_get := c_l_get_lastn.comp₂ left (c_sub.comp₂ (c_pred.comp (left.comp left)) (right))
-@[simp] theorem c_l_get_ev_pr:code_prim c_l_get := by unfold c_l_get; repeat (first|assumption|simp|constructor)
-@[simp] theorem c_l_get_evp:eval_prim O c_l_get = unpaired2 Nat.list_get := by
-  unfold Nat.list_get;
-  simp [c_l_get,eval_prim];
-  funext xs
-  exact rfl
-@[simp] theorem c_l_get_ev:eval O c_l_get = unpaired2 Nat.list_get := by rw [← eval_prim_eq_eval c_l_get_ev_pr]; simp only [c_l_get_evp]
-end Nat.RecursiveIn.Code
--- theorem Nat.PrimrecIn.l_get:Nat.PrimrecIn O Nat.l_get := by ...
--- theorem Nat.Primrec.l_get:Nat.Primrec Nat.l_get := by ...
-end l_get
-
--- takes a pair (list,index). returns l[i]+1 if exists, 0 otherwise
-section l_get_opt
-namespace Nat.RecursiveIn.Code
-def c_l_get_opt :=
-  let list        := left
-  let list_length := left.comp list
-  let index       := right
-
-  c_if_lt_te.comp₄ index list_length
-  (succ.comp $ c_l_get.comp₂ list index)
-  (c_const 0)
-  -- c_l_get_opt_lastn.comp₂ left (c_sub.comp₂ (c_pred.comp (left.comp left)) (right))
-@[simp] theorem c_l_get_opt_ev_pr:code_prim c_l_get_opt := by unfold c_l_get_opt; repeat (first|assumption|simp|constructor)
-@[simp] theorem c_l_get_opt_evp {O list index}:eval_prim O c_l_get_opt (Nat.pair list index) = if index<Nat.list_size list then (Nat.list_get list index)+1 else 0 := by
-  simp [c_l_get_opt,eval_prim, comp₄];
-  exact rfl
--- @[simp] theorem c_l_get_opt_ev:eval O c_l_get_opt = unpaired2 Nat.list_get := by rw [← eval_prim_eq_eval c_l_get_opt_ev_pr]; simp only [c_l_get_opt_evp]
-end Nat.RecursiveIn.Code
--- theorem Nat.PrimrecIn.l_get_opt:Nat.PrimrecIn O Nat.l_get_opt := by ...
--- theorem Nat.Primrec.l_get_opt:Nat.Primrec Nat.l_get_opt := by ...
-end l_get_opt
-
-
-@[simp] theorem Nat.list_get_last_append : Nat.list_get_last (Nat.list_append lst x) = x := by
-  unfold list_append
-  unfold list_get_last
-  simp
-
-
-
-section efl
-namespace Nat.RecursiveIn.Code
-def c_efl:ℕ→ℕ:=fun c=>c_l_append.comp (pair c_id c)
--- def c_efl:=fun c=>c_l_append.comp₂ c_id c
-@[simp] theorem c_efl_ev_pr (h:code_prim c):code_prim $ c_efl c := by unfold c_efl; repeat (first|assumption|simp|constructor)
-
--- @[simp] theorem c_efl_pr_aux:Primrec (pair c_id) := by
---   refine Primrec.projection ?_
---   apply PrimrecIn.PrimrecIn₂_iff_Primrec₂.mp
---   intro O
---   apply pair_prim
--- @[simp] theorem c_efl_pr: Nat.Primrec c_efl := by
---   refine Primrec.nat_iff.mp ?_
---   apply c_efl_pr_aux
-
--- huh interesting, it doesn't care about c being code_prim or not.
-@[simp] theorem c_efl_evp:eval_prim O (c_efl c) x= Nat.list_append x (eval_prim O c x) := by
-  unfold list_append
-  simp [c_efl,eval_prim];
-  unfold list_append
-  simp
-@[simp] theorem c_efl_ev : eval O (c_efl c) x = Nat.list_append <$> x <*> (eval O c x) := by
-  unfold Nat.list_append
-  simp [c_efl,eval]
-  simp [Seq.seq]
-
-  exact Part.bind_some_eq_map x.list_append (eval O c x)
-  -- exact Part.bind_some_eq_map x.list_append (eval O (decodeCode c) x)
-end Nat.RecursiveIn.Code
--- theorem Nat.PrimrecIn.efl:Nat.PrimrecIn O Nat.efl := by ...
--- theorem Nat.Primrec.efl:Nat.Primrec Nat.efl := by ...
--- theorem c_efl_ev_left (h:(eval O c x).Dom) : eval O (left.comp $ c_efl c) x = x := by
---   have h0 : (eval O c x).get h ∈ (eval O c x) := by exact Part.get_mem h
---   have h1 : eval O c x = Part.some ((eval O c x).get h) := by exact Part.get_eq_iff_eq_some.mp rfl
-
---   simp [c_efl, eval]
---   rw [h1]
---   -- should maybe define some theorem that simplfies the Nat.pair <*> business
---   simp [Seq.seq]
---   exact Part.Dom.bind h fun y ↦ Part.some x
-end efl
-
-@[simp] theorem last_efl : eval_prim O (c_l_get_last.comp (c_efl c)) = eval_prim O c := by
-  simp only [eval_prim]
-  simp
+open List
 
 
 section efl_prec
@@ -161,95 +12,20 @@ A specialised code used as an auxiliary for `c_cov_rec`.
 Given an input of the form (x, (i, list)), the code (c_efl_prec c) computes list.append (eval c input).
 (The form above is what you would expect in the inductive case in primitive recursion.)
 -/
-def c_efl_prec:=fun c=>c_l_append.comp (pair (c_id.comp (right.comp right)) c)
+def c_efl_prec:=fun c=>c_list_concat.comp (pair (c_id.comp (right.comp right)) c)
 -- def c_efl_prec:=fun c=>c_l_append.comp₂ (c_id.comp (right.comp right)) c
 @[simp] theorem c_efl_prec_ev_pr (h:code_prim c):code_prim $ c_efl_prec c := by unfold c_efl_prec; repeat (first|assumption|simp|constructor)
-@[simp] theorem c_efl_prec_evp:eval_prim O (c_efl_prec c) x= Nat.list_append x.r.r (eval_prim O c x) := by
-  unfold list_append
-  simp [c_efl_prec,eval_prim];
-  unfold list_append
-  simp
-@[simp] theorem c_efl_prec_ev : eval O (c_efl_prec c) x = Nat.list_append <$> x.r.r <*> (eval O c x) := by
-  unfold Nat.list_append
-  simp [c_efl_prec,eval]
-  simp [Seq.seq]
-  exact Part.bind_some_eq_map (unpair (unpair x).2).2.list_append (eval O c x)
+@[simp] theorem c_efl_prec_evp:eval_prim O (c_efl_prec c) x = l2n ((n2l x.r.r).concat (eval_prim O c x)) := by
+  simp [c_efl_prec]
+-- @[simp] theorem c_efl_prec_ev : eval O (c_efl_prec c) x = Nat.list_append <$> x.r.r <*> (eval O c x) := by
+--   unfold Nat.list_append
+--   simp [c_efl_prec,eval]
+--   simp [Seq.seq]
+--   exact Part.bind_some_eq_map (unpair (unpair x).2).2.list_append (eval O c x)
 end Nat.RecursiveIn.Code
 -- theorem Nat.PrimrecIn.efl_prec:Nat.PrimrecIn O Nat.efl_prec := by ...
 -- theorem Nat.Primrec.efl_prec:Nat.Primrec Nat.efl_prec := by ...
--- theorem c_efl_prec_ev_left (h:(eval O c x).Dom) : eval O (left.comp $ c_efl_prec c) x = x := by
---   have h0 : (eval O c x).get h ∈ (eval O c x) := by exact Part.get_mem h
---   have h1 : eval O c x = Part.some ((eval O c x).get h) := by exact Part.get_eq_iff_eq_some.mp rfl
-
---   simp [c_efl_prec, eval]
---   rw [h1]
---   -- should maybe define some theorem that simplfies the Nat.pair <*> business
---   simp [Seq.seq]
---   exact Part.Dom.bind h fun y ↦ Part.some x
 end efl_prec
-
-@[simp] theorem last_efl_prec : eval_prim O (c_l_get_last.comp (c_efl c)) = eval_prim O c := by
-  simp only [eval_prim]
-  simp
-
-
-
-def Nat.list_empty := Nat.pair 0 0
-def Nat.list_singleton (ele:ℕ) := Nat.list_append Nat.list_empty ele
-namespace Nat.RecursiveIn.Code
-def c_list_singleton (ele:Code): Code := c_l_append.comp₂ Nat.list_empty ele
-end Nat.RecursiveIn.Code
-
-open Nat in
-@[simp] theorem append_empty : (list_empty.list_append x).list_get 0 = x := by
-  unfold list_empty
-  unfold list_append
-  unfold list_get
-  unfold list_get_lastn
-  unfold list_get_last_aux
-  unfold list_size
-  simp
-
-
-open Nat in
-@[simp] theorem append_get_last_aux {l:ℕ}: l.list_get_last_aux i =  (l.list_append x).list_get_last_aux (i+1) := by
-  induction i
-  ·
-    unfold list_get_last_aux
-    unfold list_get_last_aux
-    unfold list_append
-    simp
-  · expose_names
-    unfold list_append
-    unfold list_get_last_aux
-    rw [h]
-    unfold list_append
-    simp
-
-open Nat in
-@[simp] theorem append_getlastn {l:ℕ}: l.list_get_lastn i = (l.list_append x).list_get_lastn (i+1) := by
-  unfold list_get_lastn
-  rw [append_get_last_aux]
-
-open Nat in
-@[simp] theorem append_size {l:ℕ} : (l.list_append x).list_size = l.list_size +1 := by
-  unfold list_append
-  unfold list_size
-  simp
-
-open Nat in
-@[simp] theorem append_get {l:ℕ} (hi:i<l.list_size): l.list_get i = (l.list_append x).list_get i := by
-  unfold list_get
-  simp only [append_size]
-  simp
-  have hi5 : l.list_size - i - 1 = l.list_size - 1 - i := by exact Simproc.sub_add_eq_comm l.list_size i 1
-  have hi6 : l.list_size - i > 0 := by exact zero_lt_sub_of_lt hi
-  have main_rewrite : (l.list_size - 1 - i)+1 = l.list_size - i := by
-    rw [←hi5]
-    exact Nat.sub_add_cancel hi6
-
-  rw [←main_rewrite]
-  exact append_getlastn
 
 
 
@@ -273,68 +49,86 @@ inductive case: Let `l` be the list of previous values, from `j=0` to `i`
 -/
 def c_cov_rec (cf cg:Code):=
   prec
-  (c_l_append.comp₂ (c_const Nat.list_empty) (cf))
+  (c_list_concat.comp₂ c_list_nil cf)
   (c_efl_prec cg)
-@[simp] theorem c_cov_rec_evp_size_positive : 0<(eval_prim O (c_cov_rec cf cg) (Nat.pair x i)).list_size := by
+@[simp] theorem c_cov_rec_evp_size_positive : 0<(n2l (eval_prim O (c_cov_rec cf cg) (Nat.pair x i))).length := by
   unfold c_cov_rec
   simp [eval_prim]
   induction i
   · simp
   · simp
-@[simp] theorem c_cov_rec_evp_size : (eval_prim O (c_cov_rec cf cg) (Nat.pair x i)).list_size = i+1 := by
+@[simp] theorem c_cov_rec_evp_size : (n2l (eval_prim O (c_cov_rec cf cg) (Nat.pair x i))).length = i+1 := by
   unfold c_cov_rec
   simp [eval_prim]
   induction i
-  · simp; exact rfl
+  · simp;
   · simp; (expose_names; exact h)
-theorem c_cov_rec_evp_0 : eval_prim O (c_cov_rec cf cg) (Nat.pair x (i+1)) = list_append (eval_prim O (c_cov_rec cf cg) (Nat.pair x i)) (  eval_prim O cg $ Nat.pair x $ Nat.pair i $ eval_prim O (c_cov_rec cf cg) (Nat.pair x i)    ) := by
+theorem c_cov_rec_evp_0 :
+  eval_prim O (c_cov_rec cf cg) (Nat.pair x (i+1))
+    =
+  (l2n $ List.concat
+  (n2l (eval_prim O (c_cov_rec cf cg) (Nat.pair x i)))
+  (eval_prim O cg $ Nat.pair x $ Nat.pair i $ eval_prim O (c_cov_rec cf cg) (Nat.pair x i))
+  ) := by
   rw  [c_cov_rec]
   rw  [eval_prim]
   simp
-@[simp] theorem c_cov_rec_evp_4 : Nat.list_get_last (eval_prim O (c_cov_rec cf cg) (Nat.pair x 0)) = eval_prim O cf x := by
+
+@[simp] theorem c_cov_rec_evp_4 : getLastI (n2l (eval_prim O (c_cov_rec cf cg) (Nat.pair x 0))) = eval_prim O cf x := by
   unfold c_cov_rec
-  simp [eval_prim]
-@[simp] theorem c_cov_rec_evp_1 : Nat.list_get (eval_prim O (c_cov_rec cf cg) (Nat.pair x i)) 0 = eval_prim O cf x := by
+  simp [getLastI]
+@[simp] theorem c_cov_rec_evp_1 : (n2l (eval_prim O (c_cov_rec cf cg) (Nat.pair x i)))[0] = eval_prim O cf x := by
   induction i with
   | zero =>
     unfold c_cov_rec
     simp [eval_prim]
   | succ i h =>
-    rw [(@c_cov_rec_evp_0 O cf cg x i)]
-    have h0 := @c_cov_rec_evp_size_positive O cf cg x i
-    rw [←append_get h0]
+    simp [c_cov_rec_evp_0]
     exact h
 
-@[simp] theorem c_cov_rec_evp_3 : Nat.list_get_last (eval_prim O (c_cov_rec cf cg) (Nat.pair x (i+1))) = (  eval_prim O cg $ Nat.pair x $ Nat.pair i $ eval_prim O (c_cov_rec cf cg) (Nat.pair x i)    ) := by
+@[simp] theorem c_cov_rec_evp_3 :
+  getLastI
+  (eval_prim O (c_cov_rec cf cg) (Nat.pair x (i+1)))
+    =
+  (  eval_prim O cg $ Nat.pair x $ Nat.pair i $ eval_prim O (c_cov_rec cf cg) (Nat.pair x i)    )
+    := by
   rw [c_cov_rec_evp_0]
-  simp only [list_get_last_append]
+  simp
 
 theorem c_cov_rec_evp_2_aux1 :
-  Nat.list_get_last (eval_prim O (c_cov_rec cf cg) (Nat.pair x i))
+  getLastI (eval_prim O (c_cov_rec cf cg) (Nat.pair x i))
     =
-  Nat.list_get (eval_prim O (c_cov_rec cf cg) (Nat.pair x i)) i := by
-  simp [list_get_last]
-  simp [list_get]
-  simp [list_get_lastn]
-  simp [list_get_last_aux]
+  (n2l (eval_prim O (c_cov_rec cf cg) (Nat.pair x i)))[i] := by
+  rw [getLastI_eq_getLast?]
+  rw [getLast?_eq_getElem?]
+  simp [c_cov_rec_evp_size]
 theorem c_cov_rec_evp_2_aux2 (h:j≤i) :
-  Nat.list_get (eval_prim O (c_cov_rec cf cg) (Nat.pair x i)) j
+  (n2l (eval_prim O (c_cov_rec cf cg) (Nat.pair x i)))[j]'(by simp [c_cov_rec_evp_size]; grind only)
     =
-  Nat.list_get (eval_prim O (c_cov_rec cf cg) (Nat.pair x (i+1))) j
+  (n2l (eval_prim O (c_cov_rec cf cg) (Nat.pair x (i+1))))[j]'(by
+    simp [c_cov_rec_evp_size];
+    grind only
+    )
   := by
   simp [c_cov_rec_evp_0]
-  apply append_get
-  simp
-  exact lt_add_one_of_le h
+  -- exact? says
+  exact
+    getElem_append_left'
+      (Eq.mpr (_root_.id (congrArg (LT.lt j) c_cov_rec_evp_size)) (c_cov_rec_evp_2_aux2._proof_1 h))
+      [eval_prim O cg (Nat.pair x (Nat.pair i (eval_prim O (cf.c_cov_rec cg) (Nat.pair x i))))]
 
-@[simp] theorem c_cov_rec_evp_2 (h:j≤i): Nat.list_get (eval_prim O (c_cov_rec cf cg) (Nat.pair x i)) j =  Nat.list_get_last (eval_prim O (c_cov_rec cf cg) (Nat.pair x j)):= by
+@[simp] theorem c_cov_rec_evp_2 (h:j≤i):
+  (n2l (eval_prim O (c_cov_rec cf cg) (Nat.pair x i)))[j]'(by simp [c_cov_rec_evp_size]; grind only)
+    = 
+  getLastI (eval_prim O (c_cov_rec cf cg) (Nat.pair x j)) := by
+
   rw [c_cov_rec_evp_2_aux1]
   induction i with
-  | zero => rw [show j=0 from eq_zero_of_le_zero h]
+  | zero => simp only [show j=0 from eq_zero_of_le_zero h]
   | succ n ih =>
     have h0: j=n+1 ∨ j≤n := by exact Or.symm (le_or_eq_of_le_succ h)
     cases h0 with
-    | inl h1 => rw [h1]
+    | inl h1 => simp only [h1]
     | inr h1 =>
       have h2 := ih h1
       rw [←h2]
@@ -397,6 +191,7 @@ def c_div_flip_aux :=
   let divisor := left
   let list_of_prev_values := right.comp right
 
+
   c_cov_rec
 
   (c_const 0) $            -- base case: if dividend is 0, return 0
@@ -404,9 +199,9 @@ def c_div_flip_aux :=
   c_ifz.comp₂ divisor $    -- in general, test if the divisor is zero
   pair (c_const 0) $       -- if so, return 0
   c_if_lt_te.comp₄ dividend divisor (c_const 0) $ -- if dividend < divisor, return 0
-  (succ.comp (c_l_get.comp₂ list_of_prev_values (c_sub.comp₂ dividend divisor))) -- else return (dividend-divisor)/divisor+1
-def c_div_flip := c_l_get_last.comp c_div_flip_aux
-def c_div := c_div_flip.comp (pair right left)
+  (succ.comp (c_list_getI.comp₂ list_of_prev_values (c_sub.comp₂ dividend divisor))) -- else return (dividend-divisor)/divisor+1
+def c_div_flip := c_list_getLastI.comp c_div_flip_aux
+def c_div := c_div_flip.comp (c_flip)
 -- i want the inductive case to be simplified to an expression involving c_div_flip2.
 -- this cannot be done after unfolding c_div_flip2, as that will destroy all 'c_div_flip2' 's.
 -- not sure how to do it automatically. in the meanwhile, i can explicitly define it, like below:
@@ -418,7 +213,54 @@ theorem c_div_flip_evp_aux_aux :
   if n<d then 0 else eval_prim O c_div_flip (Nat.pair (d+1) (n-d)) + 1
     := by
 
-  unfold c_div_flip; simp only [eval_prim, c_l_get_last_evp] -- unwrap the list_get_last wrapper
+  -- unfold c_div_flip;
+  -- unfold c_div_flip_aux
+
+  rw (config:={occs:=.pos [1]}) [c_div_flip]
+  unfold c_div_flip_aux
+  -- erw (config:={occs:=.pos [1]}) [c_div_flip_aux]
+
+  lift_lets
+  extract_lets
+  expose_names
+
+  have hdivisor : eval_prim O divisor (Nat.pair (d + 1) (Nat.pair n (eval_prim O c_div_flip_aux (Nat.pair (d + 1) n)))) = d+1 := by
+    simp [divisor]
+  have hdividend : eval_prim O dividend (Nat.pair (d + 1) (Nat.pair n (eval_prim O c_div_flip_aux (Nat.pair (d + 1) n)))) = n+1 := by
+    simp [dividend]
+
+
+
+  have stupidrewrite : (eval_prim O
+              ((c_const 0).c_cov_rec
+                (c_ifz.comp
+                  (divisor.pair
+                    ((c_const 0).pair
+                      (c_if_lt_te.comp
+                        ((dividend.pair divisor).pair
+                          ((c_const 0).pair
+                            (succ.comp
+                              (c_list_getI.comp (list_of_prev_values.pair (c_sub.comp (dividend.pair divisor))))))))))))
+              (Nat.pair (d + 1) n)) = 
+              eval_prim O c_div_flip_aux (Nat.pair (d+1) (n))
+              := by exact rfl
+
+  -- set_option trace.Meta.Tactic.simp.rewrite true in
+  simp [stupidrewrite]
+  simp [hdivisor,hdividend]
+  
+  have h0: n-d≤n := by exact sub_le n d
+  -- unfold c_div_flip_aux
+  #check c_cov_rec_evp_2 h0
+  simp [c_cov_rec_evp_2 h0]
+  -- simp only [eval_prim]
+  -- simp [stupidrewrite, -eval_prim]
+
+  stop
+  -- simp
+  
+  simp only [eval_prim, c_l_get_last_evp] -- unwrap the list_get_last wrapper
+  simp only [eval_prim, c_l_get_last_evp] -- unwrap the list_get_last wrapper
 
   -- now we rewrite the expr just until it contains the expression for the list of previous calculations
   rw (config := {occs := .pos [1]}) [c_div_flip_aux]
